Limpeza com algumas adições.

theories/Nominal.v
@@ -1,33 +1,32 @@
 From Nominal Require Export Perm.
 
-Class Support A := support: A -> nameset.
+Class Support A := support: A → nameset.
 #[global] Hint Mode Support ! : typeclass_instances.
 Instance: Params (@support) 1 := {}.
 
 Section Nominal.
-  Context X `{Perm X, Spp : Support X}.
+  Context (X : Type) `{Perm X}.
 
-  Class Nominal: Prop := {
+  Class Nominal `{Spt : Support X}: Prop := {
     nperm :> Perm X;
     support_spec : ∀ (x: X) (a b: name),
-        a ∉ (support x) -> b ∉ (support x) -> [(a,b)] • x ≡@{X} x
+        a ∉ (support x) → b ∉ (support x) → [(a,b)] • x ≡@{X} x
 }.
 End Nominal.
-
-Arguments support_spec {_ _ EqN _ Nm} : rename.
+Arguments support_spec {_ PrA _ _ Nmn} : rename.
 
 (* Freshness *)
 Definition fresh_e `{Nominal X} (a: name) (x: X) :=
-  ∃ (b : name), b ∉ support x /\ [(a,b)] • x ≡@{X} x.
+  ∃ (b : name), b ∉ support x ∧ ⟨a,b⟩ • x ≡@{X} x.
 
 Definition fresh_a `{Nominal X} (a: name) (x: X) :=
-  ∀ (b : name), b ∉ support x -> [(a,b)] • x ≡@{X} x.
+  ∀ (b : name), b ∉ support x → ⟨a,b⟩ • x ≡ x.
 
 (* Infix "#" := freshness (at level 50). *)
 Infix "#ₑ" := fresh_e (at level 50).
 Infix "#ₐ" := fresh_a (at level 50).
 
-Lemma some_any `{Nominal X} (a: name) (x: X) : a #ₑ x <-> a #ₐ x.
+Lemma some_any `{Nominal X} (a: name) (x: X) : a #ₑ x ↔ a #ₐ x.
 Proof.
   split.
   - intros [b [SB HH]] c SC; destruct (decide (c = a)), (decide (c = b)); subst; auto.
@@ -39,10 +38,10 @@ Proof.
 Qed.
 
 Lemma support_fresh_e `{Nominal X} (a : name) (x: X):
-  a ∉ support x -> a #ₑ x.
+  a ∉ support x → a #ₑ x.
 Proof.
   intros; exists a; split; [idtac | rewrite swap_equiv_neutral; apply gact_id]; auto.
 Qed.
 
-Lemma support_fresh_a `{Nominal X} (a : name) (x: X): a ∉ support x -> a #ₐ x.
+Lemma support_fresh_a `{Nominal X} (a : name) (x: X): a ∉ support x → a #ₐ x.
 Proof. intros; apply some_any, support_fresh_e; auto. Qed.
