theories/Atom.v
@@ -4,6 +4,7 @@ From stdpp Require Import listset countable infinite.
 Module Type ATOMIC.
   Parameter t : Set.
 
+  (* Contable? *)
   Axiom dec : EqDecision t.
   Axiom inf : Infinite t.
 End ATOMIC.
@@ -16,19 +17,9 @@ Module Atom : ATOMIC.
 End Atom.
 #[global] Existing Instances Atom.dec Atom.inf.
 
+
+(* Elpi experiments name *)
 From elpi Require Import elpi.
-
-(* Class Atomic A := { dec :> EqDecision A; inf :> Infinite A }.
-Global Hint Mode Atomic ! : typeclass_instances.
-Arguments dec {_ _} _ _ : simpl never, assert.
-Arguments inf {_ _} : simpl never, assert.
-
-Definition Name : Set := nat.
-Instance name_atomic : Atomic Name. Proof. split; typeclasses eauto. Qed.
-
-Arguments Name : simpl never, assert.
-#[global] Opaque Name.
-*)
 
 Elpi Db atom.sort.db lp:{{
   pred atom-sort o:id.
@@ -48,7 +39,7 @@ Elpi Accumulate declare_name lp:{{
   main _ :- coq.say "Usage: declare_name [name]".
 }}.
 Elpi Typecheck.
-
 Elpi declare_name name.
 
+(* Finite set of names *)
 Notation nameset := (listset name).
